updates

generic/Zeta.Generic.Thread.fsti
@@ -1,10 +1,12 @@
 module Zeta.Generic.Thread
 
-open Zeta.GenericVerifier
 open Zeta.Time
+open Zeta.MultiSetHashDomain
+open Zeta.GenericVerifier
 
 module S = FStar.Seq
 module SA = Zeta.SeqAux
+module MSD = Zeta.MultiSetHashDomain
 
 (* a verifier log attached to a thread id *)
 let tid_vlog (vspec: verifier_spec) = thread_id & verifier_log vspec
@@ -61,3 +63,32 @@ val lemma_state_transition (#vspec:verifier_spec) (tl: verifiable_log vspec) (i:
   Lemma (ensures (state_at tl (i + 1) ==
                   verify_step (index tl i) (state_at tl i)))
         [SMTPat (verify_step (index tl i) (state_at tl i))]
+
+val blum_add_seq (#vspec: verifier_spec) (ep: epoch) (tl: verifiable_log vspec):
+  S.seq (ms_hashfn_dom vspec.app)
+
+(* map a blum add to an index of the add sequence of the epoch of the add *)
+val add_seq_map
+  (#vspec: verifier_spec)
+  (tl: verifiable_log vspec)
+  (i: seq_index tl {is_blum_add (index tl i)}):
+  (let be = blum_add_elem (index tl i) in
+   let ep = epoch_of be in
+   let add_seq = blum_add_seq ep tl in
+   j: SA.seq_index add_seq{S.index add_seq j = be})
+
+val add_seq_inv_map
+  (#vspec: verifier_spec)
+  (ep: epoch)
+  (tl: verifiable_log vspec)
+  (j: SA.seq_index (blum_add_seq ep tl)):
+  (i: seq_index tl {is_blum_add (index tl i) /\
+                    blum_add_elem (index tl i) = S.index (blum_add_seq ep tl) j /\
+                    epoch_of (blum_add_elem (index tl i)) = ep /\
+                    add_seq_map tl i = j})
+
+val lemma_add_seq_inv (#vspec:_) (tl: verifiable_log vspec) (i: seq_index tl{is_blum_add (index tl i)}):
+  Lemma (ensures (let be = blum_add_elem (index tl i) in
+                  let ep = epoch_of be in
+                  add_seq_inv_map ep tl (add_seq_map tl i) = i))
+        [SMTPat (add_seq_map tl i)]
